% Generated by xcas
\documentclass{article} 
 \usepackage{pstricks} 
 \begin{document} 
\begin{equation} \label{eq:0}
\mbox{assume}(Ax=(-1)) = \mbox{parameter}(By,-4.200000,4.200000,0.955000)
\end{equation}
\begin{equation} \label{eq:1}
\mbox{assume}(Ay=(-1)) = \mbox{parameter}(Ay,-4.200000,4.200000,-1)
\end{equation}
\begin{equation} \label{eq:2}
A:=\mbox{point}(Ax,Ay) = \mbox{pnt}(Ax+i\* Ay,0,\mbox{A})
\end{equation}
\begin{equation} \label{eq:3}
\mbox{assume}(Bx=0.500000) = \mbox{parameter}(Bx,-4.200000,4.200000,0.500000)
\end{equation}
\begin{equation} \label{eq:4}
\mbox{assume}(By=0.764000) = \mbox{parameter}(By,-4.200000,4.200000,0.764000)
\end{equation}
\begin{equation} \label{eq:5}
B:=\mbox{point}(Bx,By) = \mbox{pnt}(Bx+i\* By,0,\mbox{B})
\end{equation}
\begin{equation} \label{eq:6}
\mbox{assume}(Cx=1) = \mbox{parameter}(Cx,-4.200000,4.200000,1)
\end{equation}
\begin{equation} \label{eq:7}
\mbox{assume}(Cy=(-1)) = \mbox{parameter}(Cy,-4.200000,4.200000,-1)
\end{equation}
\begin{equation} \label{eq:8}
C:=\mbox{point}(Cx,Cy) = \mbox{pnt}(Cx+i\* Cy,0,\mbox{C})
\end{equation}
\begin{equation} \label{eq:9}
\mbox{triangle}(A,B,C) = \mbox{pnt}(pnt[group[Ax+i\* Ay,Bx+i\* By,Cx+i\* Cy,Ax+i\* Ay],0])
\end{equation}
\begin{equation} \label{eq:10}
a:=\mbox{mediatrice}(A,B) = \mbox{pnt}(pnt[line[-By+Ay+i\* (Bx-Ax)+\frac{(Ax+i\* Ay+Bx+i\* By)}{2},By-Ay-(i\* (Bx-Ax))+\frac{(Ax+i\* Ay+Bx+i\* By)}{2}],0,\mbox{a}])
\end{equation}
\begin{equation} \label{eq:11}
b:=\mbox{mediatrice}(B,C) = \mbox{pnt}(pnt[line[-Cy+By+i\* (Cx-Bx)+\frac{(Bx+i\* By+Cx+i\* Cy)}{2},Cy-By-(i\* (Cx-Bx))+\frac{(Bx+i\* By+Cx+i\* Cy)}{2}],0,\mbox{b}])
\end{equation}
\begin{equation} \label{eq:12}
c:=\mbox{mediatrice}(C,A) = \mbox{pnt}(pnt[line[-Ay+Cy+i\* (Ax-Cx)+\frac{(Cx+i\* Cy+Ax+i\* Ay)}{2},Ay-Cy-(i\* (Ax-Cx))+\frac{(Cx+i\* Cy+Ax+i\* Ay)}{2}],0,\mbox{c}])
\end{equation}
\begin{equation} \label{eq:13}
M:=\mbox{head}(\mbox{inter}(a,b)) = \mbox{pnt}(\frac{(-(By^{2}\* Ay)-(-i\* By^{2}\* Ax)-(i\* By^{2}\* Cx)+By^{2}\* Cy+By\* (Ay)^{2}+By\* (Ax)^{2}-(By\* Cx^{2})-(By\* (Cy)^{2})-(i\* (Ay)^{2}\* Bx)-(-i\* (Ay)^{2}\* Cx)-((Ay)^{2}\* Cy)-(Ay\* Bx^{2})+Ay\* Cx^{2}+Ay\* (Cy)^{2}-(-i\* Bx^{2}\* Ax)-(i\* Bx^{2}\* Cx)+Bx^{2}\* Cy-(i\* Bx\* (Ax)^{2})-(-i\* Bx\* Cx^{2})-(-i\* Bx\* (Cy)^{2})-(-i\* (Ax)^{2}\* Cx)-((Ax)^{2}\* Cy)-(i\* Ax\* Cx^{2})-(i\* Ax\* (Cy)^{2}))}{(2\* By\* Ax+-2\* By\* Cx+-2\* Ay\* Bx+2\* Ay\* Cx+2\* Bx\* Cy+-2\* Ax\* Cy)},0,\mbox{M})
\end{equation}
\begin{equation} \label{eq:14}
N:=\mbox{head}(\mbox{inter}(b,c)) = \mbox{pnt}(\frac{(-((Cy)^{2}\* By)-(-i\* (Cy)^{2}\* Bx)-(i\* (Cy)^{2}\* Ax)+(Cy)^{2}\* Ay+Cy\* By^{2}+Cy\* Bx^{2}-(Cy\* (Ax)^{2})-(Cy\* (Ay)^{2})-(i\* By^{2}\* Cx)-(-i\* By^{2}\* Ax)-(By^{2}\* Ay)-(By\* Cx^{2})+By\* (Ax)^{2}+By\* (Ay)^{2}-(-i\* Cx^{2}\* Bx)-(i\* Cx^{2}\* Ax)+Cx^{2}\* Ay-(i\* Cx\* Bx^{2})-(-i\* Cx\* (Ax)^{2})-(-i\* Cx\* (Ay)^{2})-(-i\* Bx^{2}\* Ax)-(Bx^{2}\* Ay)-(i\* Bx\* (Ax)^{2})-(i\* Bx\* (Ay)^{2}))}{(2\* Cy\* Bx+-2\* Cy\* Ax+-2\* By\* Cx+2\* By\* Ax+2\* Cx\* Ay+-2\* Bx\* Ay)},0,\mbox{N})
\end{equation}
\begin{equation} \label{eq:15}
\mbox{normal}(\mbox{longueur2}(M,N)) = 0
\end{equation}

\end{document}
